theories/core/utp_pred.thy
@@ -72,7 +72,7 @@ definition EqualsP ::
    'VALUE WF_PREDICATE" where
 "EqualsP v x = LiftP (\<lambda> b . \<langle>b\<rangle>\<^sub>bv = x)"
 
-notation EqualsP (infix "=p" 210)
+notation EqualsP (infix "=\<^sub>p" 210)
 
 subsubsection {* True and False *}
 
@@ -93,7 +93,7 @@ lift_definition NotP ::
    'VALUE WF_PREDICATE" 
 is "uminus" .
 
-notation NotP ("\<not>p _" [190] 190)
+notation NotP ("\<not>\<^sub>p _" [190] 190)
 
 lift_definition AndP ::
   "'VALUE WF_PREDICATE \<Rightarrow>
@@ -101,7 +101,7 @@ lift_definition AndP ::
    'VALUE WF_PREDICATE" 
 is "op \<inter> :: 'VALUE WF_BINDING set \<Rightarrow> 'VALUE WF_BINDING set \<Rightarrow> 'VALUE WF_BINDING set" .
 
-notation AndP (infixr "\<and>p" 180)
+notation AndP (infixr "\<and>\<^sub>p" 180)
 
 lift_definition OrP ::
   "'VALUE WF_PREDICATE \<Rightarrow>
@@ -109,23 +109,23 @@ lift_definition OrP ::
    'VALUE WF_PREDICATE" 
 is "op \<union> :: 'VALUE WF_BINDING set \<Rightarrow> 'VALUE WF_BINDING set \<Rightarrow> 'VALUE WF_BINDING set" .
 
-notation OrP (infixr "\<or>p" 170)
+notation OrP (infixr "\<or>\<^sub>p" 170)
 
 definition ImpliesP ::
   "'VALUE WF_PREDICATE \<Rightarrow>
    'VALUE WF_PREDICATE \<Rightarrow>
    'VALUE WF_PREDICATE" where
-"ImpliesP p1 p2 = \<not>p p1 \<or>p p2"
+"ImpliesP p1 p2 = \<not>\<^sub>p p1 \<or>\<^sub>p p2"
 
-notation ImpliesP (infixr "\<Rightarrow>p" 160)
+notation ImpliesP (infixr "\<Rightarrow>\<^sub>p" 160)
 
 definition IffP ::
   "'VALUE WF_PREDICATE \<Rightarrow>
    'VALUE WF_PREDICATE \<Rightarrow>
    'VALUE WF_PREDICATE" where
-"IffP p1 p2 \<equiv> (p1 \<Rightarrow>p p2) \<and>p (p2 \<Rightarrow>p p1)"
+"IffP p1 p2 \<equiv> (p1 \<Rightarrow>\<^sub>p p2) \<and>\<^sub>p (p2 \<Rightarrow>\<^sub>p p1)"
 
-notation IffP (infixr "\<Leftrightarrow>p" 150)
+notation IffP (infixr "\<Leftrightarrow>\<^sub>p" 150)
 
 subsubsection {* Quantifiers *}
 
@@ -135,24 +135,24 @@ lift_definition ExistsP ::
    'VALUE WF_PREDICATE" is
 "\<lambda> vs p. {b1 \<oplus>\<^sub>b b2 on vs | b1 b2. b1 \<in> p}" .
 
-notation ExistsP ("(\<exists>p _ ./ _)" [0, 10] 10)
+notation ExistsP ("(\<exists>\<^sub>p _ ./ _)" [0, 10] 10)
 
 definition ForallP ::
   "'VALUE VAR set \<Rightarrow>
    'VALUE WF_PREDICATE \<Rightarrow>
    'VALUE WF_PREDICATE" where
-"ForallP vs p = \<not>p (\<exists>p vs . \<not>p p)"
+"ForallP vs p = \<not>\<^sub>p (\<exists>\<^sub>p vs . \<not>\<^sub>p p)"
 
-notation ForallP ("(\<forall>p _ ./ _)" [0, 10] 10)
+notation ForallP ("(\<forall>\<^sub>p _ ./ _)" [0, 10] 10)
 
 subsubsection {* Universal Closure *}
 
 definition ClosureP ::
   "'VALUE WF_PREDICATE \<Rightarrow>
    'VALUE WF_PREDICATE" where
-"ClosureP p = (\<forall>p VAR . p)"
+"ClosureP p = (\<forall>\<^sub>p VAR . p)"
 
-notation ClosureP ("[_]p")
+notation ClosureP ("[_]\<^sub>p")
 
 subsubsection {* Refinement *}
 
@@ -160,23 +160,33 @@ definition RefP ::
   "'VALUE WF_PREDICATE \<Rightarrow>
    'VALUE WF_PREDICATE \<Rightarrow>
    'VALUE WF_PREDICATE" where
-"RefP p1 p2 = [p2 \<Rightarrow>p p1]p"
+"RefP p1 p2 = [p2 \<Rightarrow>\<^sub>p p1]\<^sub>p"
 
-notation RefP (infix "\<sqsubseteq>p" 100)
+notation RefP (infix "\<sqsubseteq>\<^sub>p" 100)
 
-subsubsection {* Predicate Renaming *}
+subsubsection {* Predicate Permuation *}
 
-lift_definition RenameP ::
+lift_definition PermP ::
+  "'VALUE VAR_RENAME \<Rightarrow>
+   'VALUE WF_PREDICATE \<Rightarrow>
+   'VALUE WF_PREDICATE" is
+"\<lambda> ss p. (RenameB ss) ` p" .
+
+abbreviation RenameP ::
   "'VALUE WF_PREDICATE \<Rightarrow>
    'VALUE VAR_RENAME \<Rightarrow>
-   'VALUE WF_PREDICATE" ("_[_]" [200]) is
-"\<lambda> p ss. (RenameB ss) ` p" done
+   'VALUE WF_PREDICATE" ("_[_]\<^sub>p" [200] 200) where
+"RenameP p ss \<equiv> PermP ss p"
+
+setup {*
+Adhoc_Overloading.add_variant @{const_name permute} @{const_name PermP}
+*}
 
 definition RenamePMap :: 
   "'VALUE  WF_PREDICATE \<Rightarrow> 
    ('VALUE VAR \<rightharpoonup> 'VALUE VAR) \<Rightarrow> 
    'VALUE WF_PREDICATE" ("_\<^bsup>_\<^esup>" [200]) where
-"RenamePMap p ss \<equiv> RenameP p (MapR ss)"
+"RenamePMap p ss \<equiv> p[MapR ss]\<^sub>p"
 
 subsection {* Meta-logical Operators *}
 
@@ -184,7 +194,7 @@ subsubsection {* Tautologies *}
 
 definition Tautology ::
   "'VALUE WF_PREDICATE \<Rightarrow> bool" where
-"Tautology p \<longleftrightarrow> [p]p = true"
+"Tautology p \<longleftrightarrow> [p]\<^sub>p = true"
 
 declare [[coercion Tautology]]
 
@@ -192,7 +202,7 @@ notation Tautology ("taut _" [50] 50)
 
 definition Contradiction ::
   "'VALUE WF_PREDICATE \<Rightarrow> bool" where
-"Contradiction p \<longleftrightarrow> [p]p = false"
+"Contradiction p \<longleftrightarrow> [p]\<^sub>p = false"
 
 notation Contradiction ("contra _" [50] 50)
 
@@ -208,10 +218,10 @@ instantiation WF_PREDICATE :: (VALUE) ord
 begin
 
 definition less_eq_WF_PREDICATE :: "'a WF_PREDICATE \<Rightarrow> 'a WF_PREDICATE \<Rightarrow> bool" where
-"less_eq_WF_PREDICATE p1 p2 \<longleftrightarrow> taut (p2 \<sqsubseteq>p p1)"
+"less_eq_WF_PREDICATE p1 p2 \<longleftrightarrow> taut (p2 \<sqsubseteq>\<^sub>p p1)"
 
 definition less_WF_PREDICATE :: "'a WF_PREDICATE \<Rightarrow> 'a WF_PREDICATE \<Rightarrow> bool" where
-"less_WF_PREDICATE p1 p2 \<longleftrightarrow> taut (p2 \<sqsubseteq>p p1) \<and> \<not> taut (p1 \<sqsubseteq>p p2)"
+"less_WF_PREDICATE p1 p2 \<longleftrightarrow> taut (p2 \<sqsubseteq>\<^sub>p p1) \<and> \<not> taut (p1 \<sqsubseteq>\<^sub>p p2)"
 
 instance ..
 
