theories/tactics/utp_expr_tac.thy
@@ -23,97 +23,97 @@ subsection {* Interpretation Function *}
 
 definition EvalE ::
   "'VALUE WF_EXPRESSION \<Rightarrow>
-   'VALUE WF_BINDING \<Rightarrow> 'VALUE" ("\<lbrakk>_\<rbrakk>\<epsilon>_" [0, 1000] 51) where
+   'VALUE WF_BINDING \<Rightarrow> 'VALUE" ("\<lbrakk>_\<rbrakk>\<^sub>e_" [0, 1000] 51) where
 "EvalE e b = \<langle>e\<rangle>\<^sub>e b"
 
 theorem EvalE_type [typing, simp]:
-"e :\<^sub>e t \<Longrightarrow> \<lbrakk>e\<rbrakk>\<epsilon>b : t"
+"e :\<^sub>e t \<Longrightarrow> \<lbrakk>e\<rbrakk>\<^sub>eb : t"
   by (simp add:EvalE_def etype_rel_def)
 
 lemma EvalE_defined [defined]:
-  "\<D> v \<Longrightarrow> \<D> (\<lbrakk>v\<rbrakk>\<epsilon>b)"
+  "\<D> v \<Longrightarrow> \<D> (\<lbrakk>v\<rbrakk>\<^sub>eb)"
   by (simp add:EvalE_def Defined_WF_EXPRESSION_def)
 
 theorem EvalE_compat [typing, simp]:
-"e \<rhd>\<^sub>e t \<Longrightarrow> \<lbrakk>e\<rbrakk>\<epsilon>b \<rhd> t"
+"e \<rhd>\<^sub>e t \<Longrightarrow> \<lbrakk>e\<rbrakk>\<^sub>eb \<rhd> t"
   by (simp add:EvalE_def evar_compat_def)
 
 subsection {* Transfer Theorems *}
 
 theorem EvalE_simp [evale] :
-"e1 = e2 \<longleftrightarrow> (\<forall> b . \<lbrakk>e1\<rbrakk>\<epsilon>b = \<lbrakk>e2\<rbrakk>\<epsilon>b)"
+"e1 = e2 \<longleftrightarrow> (\<forall> b . \<lbrakk>e1\<rbrakk>\<^sub>eb = \<lbrakk>e2\<rbrakk>\<^sub>eb)"
   by (auto simp add: EvalE_def)
 
 theorem EvalE_intro :
-"\<lbrakk>(\<forall> b . \<lbrakk>e1\<rbrakk>\<epsilon>b = \<lbrakk>e2\<rbrakk>\<epsilon>b)\<rbrakk> \<Longrightarrow> e1 = e2"
+"\<lbrakk>(\<forall> b . \<lbrakk>e1\<rbrakk>\<^sub>eb = \<lbrakk>e2\<rbrakk>\<^sub>eb)\<rbrakk> \<Longrightarrow> e1 = e2"
   by (simp add: EvalE_simp)
 
 subsection {* Distribution Theorems *}
 
 theorem EvalP_EqualP [eval]:
-"\<lbrakk>e1 ==p e2\<rbrakk>b = (\<lbrakk>e1\<rbrakk>\<epsilon>b = \<lbrakk>e2\<rbrakk>\<epsilon>b)"
+"\<lbrakk>e1 ==\<^sub>p e2\<rbrakk>b = (\<lbrakk>e1\<rbrakk>\<^sub>eb = \<lbrakk>e2\<rbrakk>\<^sub>eb)"
   by (simp add:EqualP_def EvalP_def EvalE_def)
 
-theorem EvalE_VarE [evale] :
-"\<lbrakk>VarE x\<rbrakk>\<epsilon>b = \<langle>b\<rangle>\<^sub>b x"
+theorem EvalE_VarE [eval,evale] :
+"\<lbrakk>VarE x\<rbrakk>\<^sub>eb = \<langle>b\<rangle>\<^sub>b x"
   by (simp add:VarE.rep_eq EvalE_def)
 
 theorem EvalP_ExprP [eval] :
-"\<lbrakk>ExprP e\<rbrakk>b = DestBool (\<lbrakk>e\<rbrakk>\<epsilon>b)"
+"\<lbrakk>ExprP e\<rbrakk>b = DestBool (\<lbrakk>e\<rbrakk>\<^sub>eb)"
   by (simp add:ExprP_def eval EvalE_def)
 
 theorem EvalP_VarP [eval] :
 "\<lbrakk>VarP x\<rbrakk>b = DestBool (\<langle>b\<rangle>\<^sub>b x)"
   by (simp add:eval evale)
 
-theorem EvalE_LitE [evale] :
-"v : t \<Longrightarrow> \<lbrakk>LitE v\<rbrakk>\<epsilon>b = v"
+theorem EvalE_LitE [eval,evale] :
+"v : t \<Longrightarrow> \<lbrakk>LitE v\<rbrakk>\<^sub>eb = v"
   by (auto simp add: LitE_rep_eq EvalE_def)
 
-theorem EvalE_Op1E [evale] :
-"\<lbrakk> x :!\<^sub>e a; f \<in> FUNC1 a b \<rbrakk> \<Longrightarrow> \<lbrakk>Op1E f x\<rbrakk>\<epsilon>b1 = f (\<lbrakk>x\<rbrakk>\<epsilon>b1)"
+theorem EvalE_Op1E [eval,evale] :
+"\<lbrakk> x :!\<^sub>e a; f \<in> FUNC1 a b \<rbrakk> \<Longrightarrow> \<lbrakk>Op1E f x\<rbrakk>\<^sub>eb1 = f (\<lbrakk>x\<rbrakk>\<^sub>eb1)"
   by (auto simp add: Op1E_rep_eq EvalE_def)
 
-theorem EvalE_Op2E [evale] :
-"\<lbrakk> x :!\<^sub>e a; y :!\<^sub>e b; f \<in> FUNC2 a b c \<rbrakk> \<Longrightarrow> \<lbrakk>Op2E f x y\<rbrakk>\<epsilon>b1 = f (\<lbrakk>x\<rbrakk>\<epsilon>b1) (\<lbrakk>y\<rbrakk>\<epsilon>b1)"
+theorem EvalE_Op2E [eval,evale] :
+"\<lbrakk> x :!\<^sub>e a; y :!\<^sub>e b; f \<in> FUNC2 a b c \<rbrakk> \<Longrightarrow> \<lbrakk>Op2E f x y\<rbrakk>\<^sub>eb1 = f (\<lbrakk>x\<rbrakk>\<^sub>eb1) (\<lbrakk>y\<rbrakk>\<^sub>eb1)"
   by (auto simp add: Op2E_rep_eq EvalE_def)
 
-theorem EvalE_DefaultE [evale] :
-"\<lbrakk>DefaultE t\<rbrakk>\<epsilon>b = default t"
+theorem EvalE_DefaultE [eval,evale] :
+"\<lbrakk>DefaultE t\<rbrakk>\<^sub>eb = default t"
   by (auto simp add: DefaultE_def EvalE_def LitE_rep_eq)
 
-theorem EvalE_CoerceE_LitE [evale] :
-"v : t \<Longrightarrow> \<lbrakk>CoerceE (LitE v) t\<rbrakk>\<epsilon>b = v"
+theorem EvalE_CoerceE_LitE [eval,evale] :
+"v : t \<Longrightarrow> \<lbrakk>CoerceE (LitE v) t\<rbrakk>\<^sub>eb = v"
   by (auto simp add:CoerceE_def typing evale)
 
-theorem EvalE_CoerceE_ntype [evale] :
-"\<not> e :\<^sub>e t \<Longrightarrow> \<lbrakk>CoerceE e t\<rbrakk>\<epsilon>b = default t"
+theorem EvalE_CoerceE_ntype [eval,evale] :
+"\<not> e :\<^sub>e t \<Longrightarrow> \<lbrakk>CoerceE e t\<rbrakk>\<^sub>eb = default t"
   by (simp add:CoerceE_def evale)
 
-theorem EvalE_AppE [evale] :
-"\<lbrakk> f :\<^sub>e FuncType s t; v :\<^sub>e s; \<D> f \<rbrakk> \<Longrightarrow> \<lbrakk>AppE f v\<rbrakk>\<epsilon>b = DestFunc (\<lbrakk>f\<rbrakk>\<epsilon>b) (\<lbrakk>v\<rbrakk>\<epsilon>b)"
+theorem EvalE_AppE [eval,evale] :
+"\<lbrakk> f :\<^sub>e FuncType s t; v :\<^sub>e s; \<D> f \<rbrakk> \<Longrightarrow> \<lbrakk>AppE f v\<rbrakk>\<^sub>eb = DestFunc (\<lbrakk>f\<rbrakk>\<^sub>eb) (\<lbrakk>v\<rbrakk>\<^sub>eb)"
   by (simp add:EvalE_def AppE_rep_eq)
 
-theorem EvalE_SubstE [evale] :
-"\<lbrakk>SubstE f v x\<rbrakk>\<epsilon>b = \<lbrakk>f\<rbrakk>\<epsilon>(b(x :=\<^sub>b \<lbrakk>v\<rbrakk>\<epsilon>b))"
+theorem EvalE_SubstE [eval,evale] :
+"\<lbrakk>f[v/\<^sub>ex]\<rbrakk>\<^sub>eb = \<lbrakk>f\<rbrakk>\<^sub>e(b(x :=\<^sub>b \<lbrakk>v\<rbrakk>\<^sub>eb))"
   by (simp add:SubstE.rep_eq EvalE_def)
 
-theorem EvalE_TrueE [evale] :
-"\<lbrakk>TrueE\<rbrakk>\<epsilon>b = TrueV"
+theorem EvalE_TrueE [eval,evale] :
+"\<lbrakk>TrueE\<rbrakk>\<^sub>eb = TrueV"
   by (simp add:TrueE_def EvalE_LitE[OF MkBool_type])
 
-theorem EvalE_FalseE [evale] :
-"\<lbrakk>FalseE\<rbrakk>\<epsilon>b = FalseV"
+theorem EvalE_FalseE [eval,evale] :
+"\<lbrakk>FalseE\<rbrakk>\<^sub>eb = FalseV"
   by (simp add:FalseE_def EvalE_LitE[OF MkBool_type])
 
-theorem EvalE_UNREST_override [evale] :
+theorem EvalE_UNREST_override [eval,evale] :
 "\<lbrakk> UNREST_EXPR vs e \<rbrakk> \<Longrightarrow> 
-  \<lbrakk>e\<rbrakk>\<epsilon>(b \<oplus>\<^sub>b b' on vs) = \<lbrakk>e\<rbrakk>\<epsilon>b"
+  \<lbrakk>e\<rbrakk>\<^sub>e(b \<oplus>\<^sub>b b' on vs) = \<lbrakk>e\<rbrakk>\<^sub>eb"
   by (simp add:EvalE_def UNREST_EXPR_def)
 
-theorem EvalE_UNREST_assign [evale] :
+theorem EvalE_UNREST_assign [eval,evale] :
 "\<lbrakk> x \<in> vs; UNREST_EXPR vs e; v \<rhd> x \<rbrakk> \<Longrightarrow> 
-  \<lbrakk>e\<rbrakk>\<epsilon>(b(x :=\<^sub>b v)) = \<lbrakk>e\<rbrakk>\<epsilon>b"
+  \<lbrakk>e\<rbrakk>\<^sub>e(b(x :=\<^sub>b v)) = \<lbrakk>e\<rbrakk>\<^sub>eb"
   apply (auto simp add:EvalE_def UNREST_EXPR_def)
   apply (drule_tac x="b" in spec)
   apply (drule_tac x="b(x :=\<^sub>b v)" in spec)
@@ -122,17 +122,21 @@ theorem EvalE_UNREST_assign [evale] :
   apply (metis binding_override_simps(2) binding_override_simps(8))
 done
 
-theorem EvalP_UNREST_binding_equiv [evale] :
+theorem EvalP_UNREST_binding_equiv [eval,evale] :
 "\<lbrakk> UNREST_EXPR (VAR - vs) e; b1 \<cong> b2 on vs \<rbrakk> 
- \<Longrightarrow> \<lbrakk>e\<rbrakk>\<epsilon>b1 = \<lbrakk>e\<rbrakk>\<epsilon>b2"
+ \<Longrightarrow> \<lbrakk>e\<rbrakk>\<^sub>eb1 = \<lbrakk>e\<rbrakk>\<^sub>eb2"
   by (metis (mono_tags) Compl_eq_Diff_UNIV EvalE_def UNREST_EXPR_member VAR_def binding_override_equiv binding_override_minus)
   
-theorem EvalE_RenameE [evale] :
-"\<lbrakk>e[ss]\<epsilon>\<rbrakk>\<epsilon>b = \<lbrakk>e\<rbrakk>\<epsilon>(RenameB (inv\<^sub>s ss) b)"
-  by (simp add: EvalE_def RenameE.rep_eq)
+theorem EvalE_RenameE [eval,evale] :
+"\<lbrakk>ss\<bullet>e\<rbrakk>\<^sub>eb = \<lbrakk>e\<rbrakk>\<^sub>e((inv\<^sub>s ss)\<bullet>b)"
+  by (simp add: EvalE_def PermE.rep_eq)
 
-theorem EvalP_SubstP [eval] :
-  "\<lbrakk>p[v|x]\<rbrakk>b = \<lbrakk>p\<rbrakk>(b(x :=\<^sub>b \<lbrakk>v\<rbrakk>\<epsilon>b))"
+theorem EvalE_PrimeE [eval,evale] :
+"\<lbrakk>e\<acute>\<rbrakk>\<^sub>eb = \<lbrakk>e\<rbrakk>\<^sub>e((inv\<^sub>s (dash on UNDASHED))\<bullet>b)"
+  by (simp add:PrimeE_def evale)
+
+theorem EvalP_SubstP [eval,eval] :
+  "\<lbrakk>p[v/\<^sub>px]\<rbrakk>b = \<lbrakk>p\<rbrakk>(b(x :=\<^sub>b \<lbrakk>v\<rbrakk>\<^sub>eb))"
   by (simp add:SubstP_def EvalP_def EvalE_def)
 
 (*
@@ -141,8 +145,8 @@ theorem EvalP_SubstP [eval] :
 proof -
 
   from assms(1) have "\<And> x'. is_SubstP_var p v x x' \<Longrightarrow> 
-                       \<lbrakk>SubstP_body p v x x'\<rbrakk>b = \<lbrakk>p\<rbrakk>(b(x :=\<^sub>b \<lbrakk>v\<rbrakk>\<epsilon>b))"
-    apply (subgoal_tac "b(x :=\<^sub>b \<lbrakk>v\<rbrakk>\<epsilon>b, x' :=\<^sub>b \<langle>b\<rangle>\<^sub>b x) \<oplus>\<^sub>b b on {x'} = b(x :=\<^sub>b \<lbrakk>v\<rbrakk>\<epsilon>b)")
+                       \<lbrakk>SubstP_body p v x x'\<rbrakk>b = \<lbrakk>p\<rbrakk>(b(x :=\<^sub>b \<lbrakk>v\<rbrakk>\<^sub>eb))"
+    apply (subgoal_tac "b(x :=\<^sub>b \<lbrakk>v\<rbrakk>\<^sub>eb, x' :=\<^sub>b \<langle>b\<rangle>\<^sub>b x) \<oplus>\<^sub>b b on {x'} = b(x :=\<^sub>b \<lbrakk>v\<rbrakk>\<^sub>eb)")
     apply (drule_tac b="b" in EvalE_compat)
     apply (simp add:SubstP_body_def)
 (*    apply (simp add:is_SubstP_var_def, clarify) *)
@@ -151,9 +155,9 @@ proof -
     apply (simp add:is_SubstP_var_def, clarify)
     apply (simp add:eval evale closure)
 (*    apply (simp add:is_SubstP_var_def UNREST_def, clarify) *)
-    apply (subgoal_tac "\<lbrakk>v\<rbrakk>\<epsilon> (b(x' :=\<^sub>b \<langle>b'\<rangle>\<^sub>b x')) = \<langle>v\<rangle>\<^sub>e b")
+    apply (subgoal_tac "\<lbrakk>v\<rbrakk>\<^sub>e (b(x' :=\<^sub>b \<langle>b'\<rangle>\<^sub>b x')) = \<langle>v\<rangle>\<^sub>e b")
     apply (simp add:UNREST_def binding_upd_twist)
-    apply (drule_tac x="b(x :=\<^sub>b \<lbrakk>v\<rbrakk>\<epsilon>b, x' :=\<^sub>b \<langle>b\<rangle>\<^sub>b x)" in bspec)
+    apply (drule_tac x="b(x :=\<^sub>b \<lbrakk>v\<rbrakk>\<^sub>eb, x' :=\<^sub>b \<langle>b\<rangle>\<^sub>b x)" in bspec)
     apply (simp add:EvalP_def EvalE_def)
     apply (simp add:binding_upd_twist)
   sorry
@@ -163,7 +167,7 @@ proof -
     apply (simp add:binding_upd_twist)
     apply (simp add:EvalE_def UNREST_EXPR_def)
     apply (metis)
-    apply (rule_tac x="b(x' :=\<^sub>b \<lbrakk>v\<rbrakk>\<epsilon>b)" in exI)
+    apply (rule_tac x="b(x' :=\<^sub>b \<lbrakk>v\<rbrakk>\<^sub>eb)" in exI)
     apply (simp add:is_SubstP_var_def eval evale closure binding_upd_twist)
     apply (rule conjI)
     apply (simp_all add:EvalP_def EvalE_def UNREST_def var_compat_def)
@@ -189,7 +193,7 @@ qed
 *)
 
 lemma EvalE_UNREST_binding_upd [evale]:
-  "\<lbrakk> v \<rhd> x; UNREST_EXPR {x} e \<rbrakk> \<Longrightarrow> \<lbrakk>e\<rbrakk>\<epsilon>(b(x :=\<^sub>b v)) = \<lbrakk>e\<rbrakk>\<epsilon>b"
+  "\<lbrakk> v \<rhd> x; UNREST_EXPR {x} e \<rbrakk> \<Longrightarrow> \<lbrakk>e\<rbrakk>\<^sub>e(b(x :=\<^sub>b v)) = \<lbrakk>e\<rbrakk>\<^sub>eb"
   by (auto simp add:EvalE_def UNREST_EXPR_def, smt binding_upd_apply)
 
 subsection {* Proof Tactics *}
@@ -218,15 +222,15 @@ method_setup utp_expr_tac = {*
 subsection {* Proof Experiments *}
 
 theorem EqualP_trans:
-"taut (((e1 ==p e2) \<and>p (e2 ==p e3)) \<Rightarrow>p (e1 ==p e3))"
+"taut (((e1 ==\<^sub>p e2) \<and>\<^sub>p (e2 ==\<^sub>p e3)) \<Rightarrow>\<^sub>p (e1 ==\<^sub>p e3))"
   by utp_pred_tac
 
 theorem EqualP_sym:
-"(e1 ==p e2) = (e2 ==p e1)"
+"(e1 ==\<^sub>p e2) = (e2 ==\<^sub>p e1)"
   by utp_pred_auto_tac
 
 (* These need adapting for strictness *)
-theorem VarE_subst: "\<lbrakk> v :\<^sub>e vtype x; \<not> aux x \<rbrakk> \<Longrightarrow> VarE x[v|x] = v"
+theorem VarE_subst: "\<lbrakk> v :\<^sub>e vtype x; \<not> aux x \<rbrakk> \<Longrightarrow> $\<^sub>ex[v/\<^sub>ex] = v"
   by utp_expr_tac
 
 theorem EvalP_UNREST_assign_1 [eval] :
@@ -237,7 +241,8 @@ theorem EvalP_UNREST_assign_1 [eval] :
 done
 
 lemma ExistsP_SubstP:
-  "\<lbrakk> vtype x = vtype y; aux x = aux y; UNREST {x} p \<rbrakk> \<Longrightarrow> (\<exists>p {y}. p) = (\<exists>p {x}. p[VarE x|y])"
+  "\<lbrakk> vtype x = vtype y; aux x = aux y; UNREST {x} p \<rbrakk> \<Longrightarrow> 
+     (\<exists>\<^sub>p {y}. p) = (\<exists>\<^sub>p {x}. p[$\<^sub>ex/\<^sub>py])"
   apply (simp add:eval evale typing defined unrest binding_upd_twist)
   apply (clarify)
   apply (rule, erule exE)
@@ -252,7 +257,7 @@ done
 
 (*
   apply (auto)
-  apply (drule_tac v="\<lbrakk>e\<rbrakk>\<epsilon>b" and b="b" in EvalE_UNREST_assign[of x "{x}" e, simplified])
+  apply (drule_tac v="\<lbrakk>e\<rbrakk>\<^sub>eb" and b="b" in EvalE_UNREST_assign[of x "{x}" e, simplified])
   apply (simp_all)
 done
 *)
