theories/laws/utp_pred_laws.thy
@@ -13,128 +13,127 @@ imports
   "../core/utp_expr"
   "../tactics/utp_pred_tac"
   "../tactics/utp_expr_tac"
-  "../parser/utp_pred_parser"
   utp_subst_laws
 begin
 
 subsubsection {* Boolean Algebra laws *}
 
 theorem AndP_comm :
-"`p1 \<and> p2` = `p2 \<and> p1`"
+"p1 \<and>\<^sub>p p2 = p2 \<and>\<^sub>p p1"
   by (utp_pred_auto_tac)
 
 theorem AndP_idem [simp]:
-"`p \<and> p` = p"
+"p \<and>\<^sub>p p = p"
   by (utp_pred_auto_tac)
 
 theorem AndP_assoc :
-"`p1 \<and> (p2 \<and> p3)` = `(p1 \<and> p2) \<and> p3`"
+"p1 \<and>\<^sub>p (p2 \<and>\<^sub>p p3) = (p1 \<and>\<^sub>p p2) \<and>\<^sub>p p3"
   by (utp_pred_auto_tac)
 
 theorem AndP_OrP_distl :
-"`p1 \<and> (p2 \<or> p3)` = `(p1 \<and> p2) \<or> (p1 \<and> p3)`"
+"p1 \<and>\<^sub>p (p2 \<or>\<^sub>p p3) = (p1 \<and>\<^sub>p p2) \<or>\<^sub>p (p1 \<and>\<^sub>p p3)"
   by (utp_pred_auto_tac)
 
 theorem AndP_OrP_distr:
-"`(p1 \<or> p2) \<and> p3` = `(p1 \<and> p3) \<or> (p2 \<and> p3)`"
+"(p1 \<or>\<^sub>p p2) \<and>\<^sub>p p3 = (p1 \<and>\<^sub>p p3) \<or>\<^sub>p (p2 \<and>\<^sub>p p3)"
   by (utp_pred_auto_tac)
 
 theorem OrP_comm :
-"`p1 \<or> p2` = `p2 \<or> p1`"
+"p1 \<or>\<^sub>p p2 = p2 \<or>\<^sub>p p1"
   by (utp_pred_auto_tac)
 
 theorem OrP_idem [simp]:
-"`p \<or> p` = p"
+"p \<or>\<^sub>p p = p"
   by (utp_pred_auto_tac)
 
 theorem OrP_assoc :
-"`p1 \<or> (p2 \<or> p3)` = `(p1 \<or> p2) \<or> p3`"
+"p1 \<or>\<^sub>p (p2 \<or>\<^sub>p p3) = (p1 \<or>\<^sub>p p2) \<or>\<^sub>p p3"
   by (utp_pred_auto_tac)
 
 theorem OrP_AndP_distl :
-"`p1 \<or> (p2 \<and> p3)` = `(p1 \<or> p2) \<and> (p1 \<or> p3)`"
+"p1 \<or>\<^sub>p (p2 \<and>\<^sub>p p3) = (p1 \<or>\<^sub>p p2) \<and>\<^sub>p (p1 \<or>\<^sub>p p3)"
   by (utp_pred_auto_tac)
 
 theorem OrP_AndP_distr :
-"`(p1 \<and> p2) \<or> p3` = `(p1 \<or> p3) \<and> (p2 \<or> p3)`"
+"(p1 \<and>\<^sub>p p2) \<or>\<^sub>p p3 = (p1 \<or>\<^sub>p p3) \<and>\<^sub>p (p2 \<or>\<^sub>p p3)"
   by (utp_pred_auto_tac)
 
 theorem AndP_contra :
-"`p \<and> \<not> p` = false"
+"p \<and>\<^sub>p \<not>\<^sub>p p = false"
   by (utp_pred_auto_tac)
 
 theorem OrP_excluded_middle :
-"p \<or>p \<not>p p = true"
+"p \<or>\<^sub>p \<not>\<^sub>p p = true"
   by (utp_pred_auto_tac)
 
 theorem OrP_ref :
-"`p1 \<or> p2` \<sqsubseteq> p1"
+"p1 \<or>\<^sub>p p2 \<sqsubseteq> p1"
   by (utp_pred_auto_tac)
 
-lemma demorgan1: "`\<not>(x \<or> y)` = `\<not>x \<and> \<not>y`"
+lemma demorgan1: "\<not>\<^sub>p(x \<or>\<^sub>p y) = \<not>\<^sub>px \<and>\<^sub>p \<not>\<^sub>py"
   by (utp_pred_auto_tac)
 
-lemma demorgan2: "`\<not>(x \<and> y)` = `\<not>x \<or> \<not>y`"
+lemma demorgan2: "\<not>\<^sub>p(x \<and>\<^sub>p y) = \<not>\<^sub>px \<or>\<^sub>p \<not>\<^sub>py"
   by (utp_pred_auto_tac)
 
-lemma demorgan3: "`x \<or> y` = `\<not>(\<not>x \<and> \<not>y)`"
+lemma demorgan3: "x \<or>\<^sub>p y = \<not>\<^sub>p(\<not>\<^sub>px \<and>\<^sub>p \<not>\<^sub>py)"
   by (utp_pred_auto_tac)
 
 lemma utp_pred_simps [simp]:
-  "`\<not> false`    = true"
-  "`\<not> true`     = false"
-  "`\<not> \<not> p` = p"
-  "`false \<and> x`  = false" 
-  "`x \<and> false`  = false"
-  "`true \<and> x`   = x"
-  "`x \<and> true`   = x"
-  "`true \<or> x`   = true"
-  "`x \<or> true`   = true"
-  "`false \<or> x`  = x"
-  "`x \<or> false`  = x"
-  "`false \<Rightarrow> x` = true" 
-  "`true \<Rightarrow> x`  = x" 
-  "`p \<Rightarrow> true` = true" 
-  "`p \<Rightarrow> false` = `\<not> p`"
-  "`P \<Leftrightarrow> true` = `P`" 
-  "`true \<Leftrightarrow> P` = `P`" 
-  "`P \<Leftrightarrow> false` = `\<not> P`" 
-  "`false \<Leftrightarrow> P` = `\<not> P`" 
+  "\<not>\<^sub>p false    = true"
+  "\<not>\<^sub>p true     = false"
+  "\<not>\<^sub>p \<not>\<^sub>p p = p"
+  "false \<and>\<^sub>p x  = false" 
+  "x \<and>\<^sub>p false  = false"
+  "true \<and>\<^sub>p x   = x"
+  "x \<and>\<^sub>p true   = x"
+  "true \<or>\<^sub>p x   = true"
+  "x \<or>\<^sub>p true   = true"
+  "false \<or>\<^sub>p x  = x"
+  "x \<or>\<^sub>p false  = x"
+  "false \<Rightarrow>\<^sub>p x = true" 
+  "true \<Rightarrow>\<^sub>p x  = x" 
+  "p \<Rightarrow>\<^sub>p true = true" 
+  "p \<Rightarrow>\<^sub>p false = \<not>\<^sub>p p"
+  "P \<Leftrightarrow>\<^sub>p true = P" 
+  "true \<Leftrightarrow>\<^sub>p P = P" 
+  "P \<Leftrightarrow>\<^sub>p false = \<not>\<^sub>p P" 
+  "false \<Leftrightarrow>\<^sub>p P = \<not>\<^sub>p P" 
   by (utp_pred_tac)+
 
 subsection {* Introduction rules *}
 
-lemma RefP_OrP: "p \<sqsubseteq> q \<longleftrightarrow> p = p \<or>p q"
+lemma RefP_OrP: "p \<sqsubseteq> q \<longleftrightarrow> p = p \<or>\<^sub>p q"
   by (utp_pred_auto_tac)
 
 lemma RefP_OrP_intro [intro]:
-  "`p \<or> q` = `p` \<Longrightarrow> `p \<sqsubseteq> q`"
+  "p \<or>\<^sub>p q = p \<Longrightarrow> p \<sqsubseteq> q"
   by (utp_pred_auto_tac)
 
-lemma RefP_AndP: "p \<sqsubseteq> q \<longleftrightarrow> q = p \<and>p q"
+lemma RefP_AndP: "p \<sqsubseteq> q \<longleftrightarrow> q = p \<and>\<^sub>p q"
   by (utp_pred_auto_tac)
 
 lemma RefP_AndP_intro [intro]:
-  "`p \<and> q` = `q` \<Longrightarrow> `p \<sqsubseteq> q`"
+  "p \<and>\<^sub>p q = q \<Longrightarrow> p \<sqsubseteq> q"
   by (utp_pred_auto_tac)
 
 lemma IffP_eq_intro [intro]:
-  "`p \<Leftrightarrow> q` \<Longrightarrow> p = q"
+  "p \<Leftrightarrow>\<^sub>p q \<Longrightarrow> p = q"
   by (utp_pred_auto_tac)
 
 lemma ClosureP_intro: 
-  "`[p]` \<Longrightarrow> taut p"
+  "[p]\<^sub>p \<Longrightarrow> taut p"
   by (utp_pred_tac)
 
 subsection {* Implication Laws *}
 
 lemma ImpliesP_export:
-  "`p \<Rightarrow> q` = `p \<Rightarrow> (p \<and> q)`"
+  "p \<Rightarrow>\<^sub>p q = p \<Rightarrow>\<^sub>p (p \<and>\<^sub>p q)"
   by (utp_pred_tac)
 
 lemma ImpliesP_eq_subst:
-  "v \<rhd>\<^sub>e x \<Longrightarrow> (VarE x ==p v) \<Rightarrow>p p = (VarE x ==p v) \<Rightarrow>p p[v|x]"
-  apply (utp_pred_tac, utp_expr_tac)
+  "v \<rhd>\<^sub>e x \<Longrightarrow> ($\<^sub>ex ==\<^sub>p v \<Rightarrow>\<^sub>p p) = ($\<^sub>ex ==\<^sub>p v \<Rightarrow>\<^sub>p p[v/\<^sub>px])"
+  apply (utp_pred_tac)
   apply (auto simp add:evale eval typing)
   apply (metis binding_upd_simps(2))+
 done
@@ -142,15 +141,15 @@ done
 subsection {* Quantifier Laws *}
 
 theorem ExistsP_ident :
-"\<lbrakk>UNREST vs p\<rbrakk> \<Longrightarrow> (\<exists>p vs . p) = p"
+"\<lbrakk>UNREST vs p\<rbrakk> \<Longrightarrow> (\<exists>\<^sub>p vs . p) = p"
   by (utp_pred_tac)
 
 theorem ForallP_ident :
-"\<lbrakk>UNREST vs p\<rbrakk> \<Longrightarrow> (\<forall>p vs . p) = p"
+"\<lbrakk>UNREST vs p\<rbrakk> \<Longrightarrow> (\<forall>\<^sub>p vs . p) = p"
   by (utp_pred_tac)
 
 theorem ExistsP_union :
-"(\<exists>p vs1 \<union> vs2 . p) = (\<exists>p vs1 . \<exists>p vs2 . p)"
+"(\<exists>\<^sub>p vs1 \<union> vs2 . p) = (\<exists>\<^sub>p vs1 . \<exists>\<^sub>p vs2 . p)"
 apply (utp_pred_tac)
 apply (auto)
 apply (rule_tac x = "b'" in exI)
@@ -161,51 +160,51 @@ apply (simp add: binding_override_assoc)
 done
 
 theorem ForallP_union :
-"(\<forall>p vs1 \<union> vs2 . p) = (\<forall>p vs1 . \<forall>p vs2 . p)"
+"(\<forall>\<^sub>p vs1 \<union> vs2 . p) = (\<forall>\<^sub>p vs1 . \<forall>\<^sub>p vs2 . p)"
   by (simp add: ForallP_def ExistsP_union UNREST_NotP NotP_NotP)
 
 lemma ForallP_AndP_dist: 
-  "(\<forall>p vs. p \<and>p q) = (\<forall>p vs. p) \<and>p (\<forall>p vs. q)"
+  "(\<forall>\<^sub>p vs. p \<and>\<^sub>p q) = (\<forall>\<^sub>p vs. p) \<and>\<^sub>p (\<forall>\<^sub>p vs. q)"
   by (utp_pred_auto_tac)
 
 lemma ClosureP_AndP_dist:
-  "`[p \<and> q]` = `[p] \<and> [q]`"
+  "[p \<and>\<^sub>p q]\<^sub>p = [p]\<^sub>p \<and>\<^sub>p [q]\<^sub>p"
   by (utp_pred_auto_tac)
 
 theorem ExistsP_OrP_dist:
-"(\<exists>p vs. p1 \<or>p p2) = (\<exists>p vs. p1) \<or>p (\<exists>p vs. p2)"
+"(\<exists>\<^sub>p vs. p1 \<or>\<^sub>p p2) = (\<exists>\<^sub>p vs. p1) \<or>\<^sub>p (\<exists>\<^sub>p vs. p2)"
   by (utp_pred_auto_tac)
 
 theorem ExistsP_AndP_expand1:
 "\<lbrakk>UNREST vs p2\<rbrakk> \<Longrightarrow>
- (\<exists>p vs. p1) \<and>p p2 = (\<exists>p vs. (p1 \<and>p p2))"
+ (\<exists>\<^sub>p vs. p1) \<and>\<^sub>p p2 = (\<exists>\<^sub>p vs. (p1 \<and>\<^sub>p p2))"
   by (utp_pred_tac)
 
 theorem ExistsP_AndP_expand2:
 "\<lbrakk>UNREST vs p1\<rbrakk> \<Longrightarrow>
- p1 \<and>p (\<exists>p vs. p2) = (\<exists>p vs. (p1 \<and>p p2))"
+ p1 \<and>\<^sub>p (\<exists>\<^sub>p vs. p2) = (\<exists>\<^sub>p vs. (p1 \<and>\<^sub>p p2))"
   by (utp_pred_tac)
 
 text {* The one point rule *}
 theorem ExistsP_one_point:
   "\<lbrakk> e \<rhd>\<^sub>e x; UNREST_EXPR {x} e \<rbrakk> \<Longrightarrow>
-  `\<exists> x. (p \<and> $x = e)` = `p[e/x]`"
+  (\<exists>\<^sub>p {x}. p \<and>\<^sub>p $\<^sub>ex ==\<^sub>p e) = p[e/\<^sub>px]"
   apply (auto simp add:eval evale typing defined)
-  apply (rule_tac x="b(x :=\<^sub>b \<lbrakk>e\<rbrakk>\<epsilon>b)" in exI)
+  apply (rule_tac x="b(x :=\<^sub>b \<lbrakk>e\<rbrakk>\<^sub>eb)" in exI)
   apply (simp)
 done
 
 lemma ExistsP_has_value:
-  "\<lbrakk> UNREST_EXPR {x} v; v \<rhd>\<^sub>e x \<rbrakk> \<Longrightarrow> `\<exists> x. $x = v` = `true`"
+  "\<lbrakk> UNREST_EXPR {x} v; v \<rhd>\<^sub>e x \<rbrakk> \<Longrightarrow> (\<exists>\<^sub>p {x}. $\<^sub>ex ==\<^sub>p v) = true"
   apply (utp_pred_tac, utp_expr_tac)
   apply (auto)
-  apply (rule_tac x="b(x :=\<^sub>b \<lbrakk>v\<rbrakk>\<epsilon>b)" in exI)
+  apply (rule_tac x="b(x :=\<^sub>b \<lbrakk>v\<rbrakk>\<^sub>eb)" in exI)
   apply (simp)
 done
 
 theorem ExistsP_SubstP_rename :
   "\<lbrakk> vtype x = vtype y; aux x = aux y; UNREST {x} p \<rbrakk> 
-   \<Longrightarrow> `\<exists> y. p` = `\<exists> x. p[$x/y]`"
+   \<Longrightarrow> (\<exists>\<^sub>p {y}. p) = (\<exists>\<^sub>p {x}. p[$\<^sub>ex/\<^sub>py])"
   apply (simp add:eval evale typing defined unrest binding_upd_twist)
   apply (clarify)
   apply (rule, erule exE)
@@ -222,16 +221,16 @@ subsection {* Expression theorems *}
 
 lemma VarP_EqualP_aux:
   "\<lbrakk> vtype x = BoolType; aux x \<rbrakk> \<Longrightarrow> 
-   `$x` = `$x = true`"
-  apply (utp_pred_tac, utp_expr_tac)
+   ($\<^sub>px) = ($\<^sub>ex ==\<^sub>p TrueE)"
+  apply (utp_pred_tac)
   apply (auto)
   apply (metis BOOL_SORT_class.Inverse FalseV_def MkBool_cases TrueV_def aux_defined binding_type)
 done
 
 lemma VarP_NotP_EqualP_aux:
   "\<lbrakk> vtype x = BoolType; aux x \<rbrakk> \<Longrightarrow> 
-   `\<not> $x` = `$x = false`"
-  apply (utp_pred_tac, utp_expr_tac)
+   (\<not>\<^sub>p $\<^sub>px) = $\<^sub>ex ==\<^sub>p FalseE"
+  apply (utp_pred_tac)
   apply (auto)
   apply (metis BOOL_SORT_class.Inverse FalseV_def MkBool_cases TrueV_def aux_defined binding_type)
 done
@@ -252,15 +251,15 @@ setup ucases.setup
 
 lemma BoolType_aux_var_split_taut [ucases]:
   "\<lbrakk> vtype x = BoolType; aux x \<rbrakk> \<Longrightarrow> 
-  `[p]` = `[p[false/x] \<and> p[true/x]]`"
-  apply (utp_pred_tac, utp_expr_tac) 
+  [p]\<^sub>p = [p[FalseE/\<^sub>px] \<and>\<^sub>p p[TrueE/\<^sub>px]]\<^sub>p"
+  apply (utp_pred_tac) 
   apply (metis FalseV_def MkBool_cases Rep_WF_BINDING_inverse TrueV_def aux_defined binding_type binding_upd_def fun_upd_idem_iff)
 done
 
 lemma BoolType_aux_var_split_exists [ucases]:
   "\<lbrakk> vtype x = BoolType; aux x \<rbrakk> \<Longrightarrow> 
-   `\<exists> x. P` = `P[false/x] \<or> P[true/x]`"
-  apply (utp_pred_tac, utp_expr_tac)
+   (\<exists>\<^sub>p {x}. P) = P[FalseE/\<^sub>px] \<or>\<^sub>p P[TrueE/\<^sub>px]"
+  apply (utp_pred_tac)
   apply (auto)
   apply (metis FalseV_def MkBool_cases Rep_WF_BINDING TrueV_def WF_BINDING_app_type aux_defined)
   apply (metis BOOL_SORT_class.Defined MkBool_type binding_upd_apply var_compat_def)
@@ -269,12 +268,12 @@ done
 
 lemma BoolType_aux_var_split_eq_intro [ucases]:
   assumes "vtype x = BoolType" "aux x" 
-          "`p[false/x]` = `q[false/x]`"
-          "`p[true/x]` = `q[true/x]`"
+          "p[FalseE/\<^sub>px] = q[FalseE/\<^sub>px]"
+          "p[TrueE/\<^sub>px] = q[TrueE/\<^sub>px]"
   shows "p = q"
   apply (rule IffP_eq_intro)
   apply (rule ClosureP_intro)
-  apply (unfold BoolType_aux_var_split_taut[OF assms(1) assms(2), of "`p \<Leftrightarrow> q`"])
+  apply (unfold BoolType_aux_var_split_taut[OF assms(1) assms(2), of "p \<Leftrightarrow>\<^sub>p q"])
   apply (simp add:usubst assms)
   apply (utp_pred_tac)
 done
@@ -292,18 +291,18 @@ lemma MkBool_False_compat [typing]:
 subsection {* Uniqueness Theorems *}
 
 lemma VarP_not_false [simp]:
-  "vtype x = BoolType \<Longrightarrow> `$x` \<noteq> `false`"
-  "vtype x = BoolType \<Longrightarrow>  `false` \<noteq> `$x`"
-  by (utp_pred_tac, utp_expr_tac, rule_tac x="\<B>(x :=\<^sub>b MkBool True)" in exI, simp add:typing)+
+  "vtype x = BoolType \<Longrightarrow> $\<^sub>px \<noteq> false"
+  "vtype x = BoolType \<Longrightarrow>  false \<noteq> $\<^sub>px"
+  by (utp_pred_tac, rule_tac x="\<B>(x :=\<^sub>b MkBool True)" in exI, simp add:typing)+
 
 lemma VarP_not_true [simp]:
-  "vtype x = BoolType \<Longrightarrow> `$x` \<noteq> `true`"
-  "vtype x = BoolType \<Longrightarrow>  `true` \<noteq> `$x`"
-  by (utp_pred_tac, utp_expr_tac, rule_tac x="\<B>(x :=\<^sub>b MkBool False)" in exI, simp add:typing)+
+  "vtype x = BoolType \<Longrightarrow> $\<^sub>px \<noteq> true"
+  "vtype x = BoolType \<Longrightarrow>  true \<noteq> $\<^sub>px"
+  by (utp_pred_tac, rule_tac x="\<B>(x :=\<^sub>b MkBool False)" in exI, simp add:typing)+
 
 lemma NotP_not_false [simp]:
-  "x \<noteq> `true` \<Longrightarrow> `\<not> x` \<noteq> `false`"
-  "x \<noteq> `false` \<Longrightarrow> `\<not> x` \<noteq> `true`"
+  "x \<noteq> true \<Longrightarrow> \<not>\<^sub>p x \<noteq> false"
+  "x \<noteq> false \<Longrightarrow> \<not>\<^sub>p x \<noteq> true"
   by (utp_pred_tac)+
 
 end
